src/study/Nemonuri.Study.CSharpSyntaxRewriter2.Modifier/Nemonuri.StratifiedNode.ListTheory.Properties.fst
@@ -104,3 +104,28 @@ let rec lemma_snl1_ends_with_snl2_means_snl1_ends_with_snl2_tl
     else
       lemma_snl1_ends_with_snl2_means_snl1_ends_with_snl2_tl (get_tl snl1) snl2
 
+let rec list_satisfies_for_all_predicate_means_head_and_tail_satisfy_predicate
+  (#t:eqtype) (#mlv:nat) (snl:stratified_node_list t mlv{SCons? snl})
+  (predicate:(#lv:pos -> stratified_node t lv -> Tot bool))
+  : Lemma (requires for_all snl predicate)
+          (ensures (predicate (get_hd snl)) && (for_all (get_tl snl) predicate))
+          (decreases snl)
+  = if (get_length snl = 1) then ()
+    else
+      list_satisfies_for_all_predicate_means_head_and_tail_satisfy_predicate (get_tl snl) predicate
+
+let rec list_satisfies_for_all_predicate_means_element_satisfies_predicate
+  (#t:eqtype) (#mlv:nat) (snl:stratified_node_list t mlv{SCons? snl})
+  (#lv:pos) (sn:stratified_node t lv)
+  (predicate:(#lv:pos -> stratified_node t lv -> Tot bool))
+  : Lemma (requires (for_all snl predicate) && (contains snl sn))
+          (ensures predicate sn)
+          (decreases snl)
+  = list_satisfies_for_all_predicate_means_head_and_tail_satisfy_predicate snl predicate;
+    if (get_hd_level snl) = lv && (get_hd snl) = sn then ()
+    else
+      list_satisfies_for_all_predicate_means_element_satisfies_predicate (get_tl snl) sn predicate
+      
+  
+  
+  //list_satisfies_for_all_predicate_means_head_and_tail_satisfy_predicate snl predicate
